Free magma universal properties (#155)
Added univeral properties of `evalInMagma` and `fmapFreeMagma`. (The
universal property of the latter follows directly from that of the
former!)

Closes #133.

I've written my own `isMagmaHom` predicate for the sake of this issue,
but it will need to be replaced with the "official" `MagmaHom`
implementation from #114 once it is complete. So this PR should not be
merged until that issue is resolved, and the necessary tweaks are made.

---------

Co-authored-by: Pietro Monticone <38562595+pitmonticone@users.noreply.github.com>
Co-authored-by: Shrys <shreyasss94@gmail.com>

equational_theories/FreeMagma.lean
@@ -1,5 +1,6 @@
-import equational_theories.EquationalResult
 import equational_theories.AllEquations
+import equational_theories.EquationalResult
+import equational_theories.Homomorphisms
 
 universe u
 universe v
@@ -23,13 +24,35 @@ instance FreeMagma.isMagma {α} : Magma (FreeMagma α) := ⟨ Fork ⟩
 
 namespace FreeMagma
 
-def fmapFreeMagma {α : Type u} {β : Type v} (f : α → β) : FreeMagma α → FreeMagma β
-  | Lf a => FreeMagma.Leaf (f a)
-  | lchild ⋆ rchild => FreeMagma.Fork (fmapFreeMagma f lchild) (fmapFreeMagma f rchild)
-
 def evalInMagma {α : Type u} {G : Type v} [Magma G] (f : α -> G) : FreeMagma α → G
   | Lf a => f a
   | lchild ⋆ rchild => (evalInMagma f lchild) ◇ (evalInMagma f rchild)
+
+def evalHom {α : Type u} {G : Type v} [Magma G] (f : α → G) : FreeMagma α →◇ G where
+   toFun := evalInMagma f
+   map_op' := fun _ _ ↦ refl _
+
+ def fmapFreeMagma {α : Type u} {β : Type v} (f : α → β) : FreeMagma α → FreeMagma β :=
+    evalInMagma (Lf ∘ f)
+
+ def fmapHom {α : Type u} {β : Type v} (f : α → β) : FreeMagma α →◇ FreeMagma β :=
+   evalHom (Lf ∘ f)
+
+ theorem EvalFreeMagmaUniversalProperty {α : Type u} {G : Type v} [Magma G] (f : α → G)
+    : ∀ g : FreeMagma α →◇ G, g.toFun ∘ Lf = f → evalInMagma f = g.toFun := by
+   intros g glift
+   let rec equiv : ∀ tx : FreeMagma α, evalInMagma f tx = g.toFun tx := fun tx ↦
+      match tx with
+      | FreeMagma.Leaf x => Eq.symm $ congrFun glift x
+      | FreeMagma.Fork txleft txright => Eq.trans
+         (congrArg (fun t ↦ t ◇ evalInMagma f txright) (equiv txleft)) $ Eq.trans
+         (congrArg (fun t ↦ g.toFun txleft ◇ t) (equiv txright))
+         (Eq.symm $ g.map_op' txleft txright)
+   exact (funext equiv)
+
+ theorem FmapFreeMagmaUniversalProperty {α : Type u} [Magma α] {β : Type u} (f : α → β)
+    : ∀ g : FreeMagma α →◇ FreeMagma β, g ∘ Lf = Lf ∘ f → fmapFreeMagma f = g :=
+    EvalFreeMagmaUniversalProperty (Lf ∘ f)
 
 end FreeMagma
 
